update lott to post macro refactor version

TabularTypeInterpreter/Data/Range.lean
@@ -5,7 +5,7 @@ namespace Std.Range
 def get!InverseOn (p p' : List Nat) (n : Nat) :=
   (∀ i ∈ [:n], p'.get! (p.get! i) = i) ∧ ∀ i ∈ [:n], p.get! (p'.get! i) = i
 
-theorem mem_toList_of_mem {m n i: Nat} (mem: i ∈ [m:n]): i ∈ [m:n].toList := by
+def mem_toList_of_mem {m n i: Nat} (mem: i ∈ [m:n]): i ∈ [m:n].toList := by
   have H := @mem_map_of_mem (f:=id)
   simp_all
 
@@ -44,12 +44,10 @@ theorem mem_toList_le {m} n {h: m <= n} : ∀i ∈ [m:n].toList, i < n := by
 theorem map_f_get!_eq [Inhabited α] [Inhabited β] {as : List α} {f : α → β} : [:as.length].map (fun i => f <| as.get! i) = as.map f := by
   match as with
   | [] =>
-    rw [List.length_nil, map, toList, if_neg (nomatch ·), if_neg (Nat.not_lt_of_le (Nat.le_refl _)),
-        List.map_nil, List.map_nil]
+    rw [List.length_nil, map, toList, if_neg (Nat.not_lt_of_le (Nat.le_refl _)), List.map_nil, List.map_nil]
   | a :: as' =>
-    rw [List.length_cons, map, toList, if_neg (nomatch ·), if_pos (Nat.succ_pos _), List.map_cons,
-        List.get!_cons_zero, ← map_shift (Nat.le_add_left ..), Nat.add_sub_cancel,
-        Nat.add_sub_cancel, map_eq_of_eq_of_mem fun _ _ => congrArg f <| List.get!_cons_succ .., ← map,
-        map_f_get!_eq, List.map_cons]
+    rw [List.length_cons, map, toList, if_pos (Nat.succ_pos _), List.map_cons, List.get!_cons_zero,
+        ←map, ← map_shift (Nat.le_add_left ..), Nat.add_sub_cancel, Nat.add_sub_cancel,
+        map_eq_of_eq_of_mem'' fun _ _ => congrArg f <| List.get!_cons_succ .., map_f_get!_eq, List.map_cons]
 
 end Std.Range
