TabularTypeInterpreter/F⊗⊕ω/Syntax/Environment.lean
@@ -2,22 +2,14 @@ import TabularTypeInterpreter.«F⊗⊕ω».Syntax.Term
 
 namespace TabularTypeInterpreter.«F⊗⊕ω»
 
-private
-def Environment.appendExpr : Lean.Expr :=
-  .const `TabularTypeInterpreter.«F⊗⊕ω».Environment.append []
-
-private
-def Environment.TypeVar_substExpr : Lean.Expr :=
-  .const `TabularTypeInterpreter.«F⊗⊕ω».Environment.TypeVar_subst []
-
 nosubst
 nonterminal Environment, Δ :=
   | "ε"                  : empty
   | Δ ", " a " : " K     : typeExt (id a)
   | Δ ", " x " : " A     : termExt (id x)
-  | "(" Δ ")"            : paren (desugar := return Δ)
-  | Δ ", " Δ'            : append (elab := return Lean.mkApp2 Environment.appendExpr Δ Δ')
-  | Δ " [" A " / " a "]" : subst (id a) (elab := return Lean.mkApp3 Environment.TypeVar_substExpr Δ a A)
+  | "(" Δ ")"            : paren (expand := return Δ)
+  | Δ ", " Δ'            : append (expand := return .mkCApp `TabularTypeInterpreter.«F⊗⊕ω».Environment.append #[Δ, Δ'])
+  | Δ " [" A " / " a "]" : subst (id a) (expand := return .mkCApp `TabularTypeInterpreter.«F⊗⊕ω».Environment.TypeVar_subst #[Δ, a, A])
 
 namespace Environment
 @[app_unexpander empty]
