TabularTypeInterpreter/F⊗⊕ω/Theorems.lean
@@ -8,18 +8,16 @@ open Std
 
 private
 theorem _root_.Membership.mem.inc {r : Range} (h : i ∈ r) : i ∈ { r with stop := r.stop + 1 } :=
-  ⟨h.lower, Nat.lt_add_right _ h.upper⟩
+  ⟨h.lower, Nat.lt_add_right _ h.upper, h.step⟩
 
 private
-theorem progress.sandwich {f : Nat → α} (h : i < n) : (List.map (fun j => [f j]) [0:n]).flatten =
-  (List.map (fun j => [f j]) [0:i]).flatten ++
-    f i :: (List.map (fun j => [f (j + (i + 1))]) [(i + 1) - (i + 1):n - (i + 1)]).flatten := by
-  simp only [List.map_singleton_flatten]
-  congr
+theorem progress.sandwich {f : Nat → α} (h : i < n) : [0:n].map (fun j => f j) =
+  [:i].map (fun j => f j) ++
+    f i :: [(i + 1) - (i + 1):n - (i + 1)].map (fun j => f (j + (i + 1))) := by
   rw [← List.singleton_append, Range.map_shift (Nat.le_refl _)]
   have : [f i] = List.map (fun j => f j) [i:i + 1] := by
-    rw [Range.toList, if_neg Nat.one_ne_zero, if_pos (Nat.lt_succ_self _), Range.toList,
-        if_neg Nat.one_ne_zero, if_neg (Nat.not_lt_of_le (Nat.le_refl _)), List.map, List.map]
+    rw [Range.toList, if_pos (Nat.lt_succ_self _), Range.toList,
+        if_neg (Nat.not_lt_of_le (Nat.le_refl _)), List.map, List.map]
   rw [this]
   rw [Range.map_append (Nat.le_succ _) (Nat.succ_le_of_lt h),
       Range.map_append (Nat.zero_le _) (Nat.le_of_lt h)]
@@ -32,12 +30,12 @@ theorem progress.fold {E : Nat → Term} (EtyA : ∀ i ∈ [0:n], [[ε ⊢ E@i :
   induction n
   · case zero =>
     right
-    intro _ ⟨_, lt_zero⟩
+    intro _ ⟨_, lt_zero, _⟩
     contradiction
   · case succ j ih' => match ih' (fun j mem => EtyA j mem.inc) (fun j mem => h j mem.inc) with
     | .inl ⟨i, mem, ⟨E'', toE''⟩⟩ => exact .inl ⟨i, mem.inc, ⟨E'', toE''⟩⟩
     | .inr IsValue =>
-      have jmem : j ∈ [0:j + 1] := ⟨Nat.zero_le _, Nat.lt_succ_self _⟩
+      have jmem : j ∈ [0:j + 1] := ⟨Nat.zero_le _, Nat.lt_succ_self _, Nat.mod_one _⟩
       match h j jmem with
       | .inl ⟨E'', toE''⟩ => exact .inl ⟨j, jmem, ⟨IsValue, ⟨E'', toE''⟩⟩⟩
       | .inr jIsValue =>
@@ -48,10 +46,11 @@ theorem progress.fold {E : Nat → Term} (EtyA : ∀ i ∈ [0:n], [[ε ⊢ E@i :
           rw [h]
           exact jIsValue
         · case neg h =>
-          exact IsValue i ⟨Nat.zero_le _, Nat.lt_of_le_of_ne (Nat.le_of_lt_succ mem.upper) h⟩
+          exact IsValue i
+            ⟨Nat.zero_le _, Nat.lt_of_le_of_ne (Nat.le_of_lt_succ mem.upper) h, Nat.mod_one _⟩
 
 local instance : Inhabited Value where
-  default := ⟨.prodIntro [], .prodIntro fun _ => (nomatch ·)⟩
+  default := ⟨.prodIntro [], .prodIntro nofun⟩
 in
 theorem progress (EtyA : [[ε ⊢ E : A]]) : (∃ E', [[E -> E']]) ∨ E.IsValue := by
   generalize Δeq : Environment.empty = Δ at EtyA
@@ -80,17 +79,19 @@ theorem progress (EtyA : [[ε ⊢ E : A]]) : (∃ E', [[E -> E']]) ∨ E.IsValue
       rw [this, Veq]
       exact .inl <| .intro _ <| .typeLamApp
   · case prodIntro n E' A wf E'ty ih => match progress.fold E'ty (fun i mem => ih i mem rfl) with
-    | .inl ⟨i, ⟨_, iltn⟩, IsValue, E'', toE''⟩ =>
-      let V j : Value := if h' : j < i then ⟨E' j, IsValue j ⟨Nat.zero_le _, h'⟩⟩ else default
-      rw [progress.sandwich iltn, Range.map_eq_of_eq_of_mem (fun j jmem => by
-          show [E' j] = [(V j).val]
+    | .inl ⟨i, ⟨_, iltn, _⟩, IsValue, E'', toE''⟩ =>
+      let V j : Value := if h' : j < i then
+          ⟨E' j, IsValue j ⟨Nat.zero_le _, h', Nat.mod_one _⟩⟩
+        else
+          default
+      rw [progress.sandwich iltn, Range.map_eq_of_eq_of_mem'' (fun j jmem => by
+          show E' j = (V j).val
           dsimp only [V]
           rw [dif_pos jmem.upper]
       ), Nat.sub_self]
       exact .inl <| .intro _ <| .prodIntro toE''
     | .inr IsValue =>
       exact .inr <| .prodIntro fun E Emem => by
-        rw [List.map_singleton_flatten] at Emem
         have ⟨i, imem, Eeq⟩ := Range.mem_of_mem_map Emem
         rw [Eeq]
         exact IsValue i imem
@@ -112,21 +113,27 @@ theorem progress (EtyA : [[ε ⊢ E : A]]) : (∃ E', [[E -> E']]) ∨ E.IsValue
       have ⟨n', mem, VE'', VE'_eq⟩ := VE'.eq_sumIntro_of_ty_sum E'ty
       cases VE'_eq
       match progress.fold Fty (fun i mem => ih₂ i mem rfl) with
-      | .inl ⟨j, ⟨_, jltn⟩, IsValue, F', toF'⟩ =>
-        let VF k : Value := if h' : k < j then ⟨F k, IsValue k ⟨Nat.zero_le _, h'⟩⟩ else default
-        rw [progress.sandwich jltn, Range.map_eq_of_eq_of_mem (fun j jmem => by
-          show [F j] = [(VF j).val]
+      | .inl ⟨j, ⟨_, jltn, _⟩, IsValue, F', toF'⟩ =>
+        let VF k : Value := if h' : k < j then
+            ⟨F k, IsValue k ⟨Nat.zero_le _, h', Nat.mod_one _⟩⟩
+          else
+            default
+        rw [progress.sandwich jltn, Range.map_eq_of_eq_of_mem'' (fun j jmem => by
+          show F j = (VF j).val
           dsimp only [VF]
           rw [dif_pos jmem.upper]
         ), Nat.sub_self]
         exact .inl <| .intro _ <| .sumElimR (V := VE') toF'
       | .inr FIsValue =>
-        let VF j : Value := if h : j < n then ⟨F j, FIsValue j ⟨Nat.zero_le _, h⟩⟩ else default
-        rw [List.map_singleton_flatten, Range.map_eq_of_eq_of_mem (fun i mem => by
+        let VF j : Value := if h : j < n then
+            ⟨F j, FIsValue j ⟨Nat.zero_le _, h, Nat.mod_one _⟩⟩
+          else
+            default
+        rw [Range.map_eq_of_eq_of_mem'' (fun i mem => by
           show F i = (VF i).val
           dsimp only [VF]
           rw [dif_pos mem.upper]
-        ), ← List.map_singleton_flatten]
+        )]
         exact .inl <| .intro _ <| .sumElimIntro mem
   · case equiv ih => exact ih rfl
 
@@ -366,7 +373,7 @@ theorem Typing.type_subst' (EtyA: [[ Δ, a: K, Δ' ⊢ E: A ]]) (BkiK : [[ Δ �
     unfold Function.comp at ih
     simp_all
     have ⟨A', A'eq⟩: ∃A': ℕ → «Type», ∀i, A' i = (A i).TypeVar_subst a B := ⟨λi => (A i).TypeVar_subst a B, λi => by simp⟩
-    rw [<- A'eq i]; rw [<- funext (λi => A'eq i |> congrArg (λx => [x]))] at ih
+    rw [<- A'eq i]; rw [<- funext (λi => A'eq i)] at ih
     refine .prodElim (n' := n) ih iRange
   . case sumIntro _ n Δ_ _ _ _ EtyA A'kiStar _ =>
     subst Δ_
