TabularTypeInterpreter/Semantics/ClassEnvironment/Basic.lean
@@ -1,0 +1,60 @@
+import Lott.Data.Range
+import TabularTypeInterpreter.Syntax.ClassEnvironment
+
+namespace TabularTypeInterpreter
+
+open «F⊗⊕ω»
+
+namespace ClassEnvironment
+
+variable (TC : TypeClass)
+
+def append (Γc : ClassEnvironment) : ClassEnvironment → ClassEnvironment
+  | empty => Γc
+  | ext Γc' γc => Γc.append Γc' |>.ext γc
+
+def TCDom : ClassEnvironment → List TypeClass
+  | empty => []
+  | ext Γc (.mk _ TC ..) => TC :: Γc.TCDom
+
+def memberDom : ClassEnvironment → List Member
+  | empty => []
+  | ext Γc (.mk _ _ _ m ..) => m :: Γc.memberDom
+
+end ClassEnvironment
+
+judgement_syntax TC " ≠ " TC' : TypeClass.Ne
+
+def TypeClass.Ne := _root_.Ne (α := TypeClass)
+
+judgement_syntax m " ≠ " m' : Member.Ne
+
+def Member.Ne := _root_.Ne (α := Member)
+
+judgement_syntax γc " ∈ " Γc : ClassEnvironment.In
+
+judgement ClassEnvironment.In :=
+
+─────────── head
+γc ∈ Γc, γc
+
+(</ TCₛ@i a ⇝ Aₛ@i // i in [:n] /> ⇒ TC a : κ) ↦ m : σ ⇝ A ∈ Γc
+TC ≠ TC'
+m ≠ m'
+───────────────────────────────────────────────────────────────────────────────────────────────────────────────────────────────────── ext {TC}
+(</ TCₛ@i a ⇝ Aₛ@i // i in [:n] /> ⇒ TC a : κ) ↦ m : σ ⇝ A ∈ Γc, (</ TC'ₛ@i a' ⇝ Aₛ'@i // i in [:n'] /> ⇒ TC' a' : κ') ↦ m' : σ' ⇝ A'
+
+judgement_syntax TC " : " κ " ⇝ " A " ∈ " Γc : ClassEnvironment.TCIn
+
+def ClassEnvironment.TCIn TC κ A Γc :=
+  ∃ TCₛ Aₛ n m σ, [[(</ TCₛ@i a ⇝ Aₛ@i // i in [:n] /> ⇒ TC a : κ) ↦ m : σ ⇝ A ∈ Γc]]
+
+judgement_syntax TC " ∉ " "dom" "(" Γc ")" : ClassEnvironment.TCNotInDom
+
+def ClassEnvironment.TCNotInDom TC (Γc : ClassEnvironment) := TC ∉ Γc.TCDom
+
+judgement_syntax m " ∉ " "dom" "(" Γc ")" : ClassEnvironment.MemberNotInDom
+
+def ClassEnvironment.MemberNotInDom m (Γc : ClassEnvironment) := m ∉ Γc.memberDom
+
+end TabularTypeInterpreter
