TabularTypeInterpreter/Semantics/ClassEnvironment/WellFormedness.lean
@@ -1,0 +1,23 @@
+import TabularTypeInterpreter.Semantics.Type
+
+namespace TabularTypeInterpreter
+
+judgement_syntax "⊢c " Γc : ClassEnvironment.WellFormedness
+
+judgement ClassEnvironment.WellFormedness :=
+
+──── empty
+⊢c ε
+
+⊢c Γc
+TC ∉ dom(Γc)
+m ∉ dom(Γc)
+⊢ κ ⇝ K
+∀ a, Γc; ε, a : κ ⊢ σ^a : * ⇝ A^a
+∀ a, ε, a : K ⊢ A^a : *
+</ ∀ a, Γc; ε, a : κ ⊢ TCₛ@i a : C ⇝ Aₛ@i^a // i in [:n] />
+</ ∀ a, ε, a : K ⊢ Aₛ@i^a : * // i in [:n] />
+───────────────────────────────────────────────────────────────── ext {TC}
+⊢c Γc, (</ TCₛ@i a ⇝ Aₛ@i // i in [:n] /> ⇒ TC a : κ) ↦ m : σ ⇝ A
+
+end TabularTypeInterpreter
