TabularTypeInterpreter/Semantics/InstanceEnvironment.lean
@@ -1,0 +1,15 @@
+import TabularTypeInterpreter.Semantics.ClassEnvironment.Basic
+import TabularTypeInterpreter.Syntax.InstanceEnvironment
+
+namespace TabularTypeInterpreter
+
+judgement_syntax Γc " ⊢ " Γᵢ : InstanceEnvironment.WellFormedness
+
+judgement InstanceEnvironment.WellFormedness :=
+
+─────── empty
+Γc ⊢ Γᵢ
+
+-- TODO: ext
+
+end TabularTypeInterpreter
