TabularTypeInterpreter/Theorems/Program.lean
@@ -1,0 +1,13 @@
+import TabularTypeInterpreter.Semantics.Program
+import TabularTypeInterpreter.Theorems.Term
+
+namespace TabularTypeInterpreter
+
+theorem Program.TypingingAndElaboration.soundness (pte : [[Γᵢ; Γc ⊢ pgm : σ ⇝ E]])
+  (Γcw : [[⊢c Γc]] := by exact .empty) (Γᵢw : [[Γc ⊢ Γᵢ]] := by exact .empty)
+  (σke : [[Γc; ε ⊢ σ : * ⇝ A]]) : [[ε ⊢ E : A]] := match pte with
+  | .cls .. => sorry
+  -- | .inst .. => sorry
+  | .term Mte => Mte.soundness σke Γcw Γᵢw .empty
+
+end TabularTypeInterpreter
